%-*-latex-*-
Prove the following proposition from our notes.
Proofs in later question can quote this proposition.

\textbf{Proposition 1.}
Let $\vec{u}, \vec{v}, \vec{w}$ be vectors and $\alpha, \beta \in \R$.
Then
\begin{myenumt}
\item $\vec{u} + \vec{v} = \vec{v} + \vec{u}$
\item $(\vec{u} + \vec{v}) + \vec{w} = \vec{u} + (\vec{v} + \vec{w})$
\item $\vec{u} + \vec{0} = \vec{u} = \vec{0} + \vec{u}$
\item $\alpha \cdot (\vec{u} + \vec{v}) = \alpha \cdot \vec{u} + \alpha \cdot \vec{v}$
\item $(\alpha + \beta) \cdot \vec{u} = \alpha \cdot \vec{u} + \beta \cdot \vec{u}$
\item $\vec{u} - \vec{u} = \vec{0}$ 
\item $1 \cdot \vec{u} = \vec{u}$
\item $-1 \cdot \vec{u} = -\vec{u}$
\item $0 \cdot \vec{u} = \vec{0}$
\item $\alpha \cdot (\beta \cdot \vec{u}) = (\alpha \cdot \beta) \cdot \vec{u}$  
\end{myenumt}
(Put your proofs in \verb!q01s.tex!.)
