%-*-latex-*-
\proof
In all the proofs below, by definition of 2D vectors, let
$\vec{u} = \langle a, b \rangle$,
$\vec{v} = \langle c, d \rangle$, and
$\vec{w} = \langle e, f \rangle$
where $a, b, c, d, e, f \in F$.

(a)
We have
\begin{align*}
  \vec{u} + \vec{v}
  &= \langle a, b \rangle + \langle c, d \rangle \\
  &= \langle a + c, b + d \rangle & & \text{ by definition of vector addition} \\
  &= \langle c + a, d + b\rangle & & \text{ by commutativity of $+$ of $F$} \\
  &= \langle c, d \rangle + \langle a, b \rangle & & \text{ by definition of vector addition} \\
  &= \vec{v} + \vec{u}  
\end{align*}

(b)
We have
\begin{align*}
  (\vec{u} + \vec{v}) + \vec{w}
  &=    \\
  &=    \\
  &=  
\end{align*}

(c)

(d)

(e)

(f)

(g)

(h)

(i)

(j)
\qed
